not

Semantics/Imp/Untyped/Aexp.lean
@@ -3,14 +3,14 @@ import Semantics.Imp.Untyped.Lang
 namespace Aexp
 namespace Natural
 
-inductive Step: Aexp → State → Val → Prop
-  | val: Step (val n) _ n
-  | var: Step (var x) s (s x)
+inductive step: Aexp → State → Val → Prop
+  | val: step (val n) _ n
+  | var: step (var x) s (s x)
   | add
-    (h₁: Step a s n) (h₂: Step b s m):
-    Step (add a b) s (n + m)
+    (h₁: step a s n) (h₂: step b s m):
+    step (add a b) s (n + m)
 
-notation s " ⊢ " a " ⟹ " v => Step a s v
+notation s " ⊢ " a " ⟹ " v => step a s v
 
 end Natural
 
@@ -31,14 +31,14 @@ theorem reduce.from_natural (h: s ⊢ a ⟹ n): a⇓s = n :=
 
 theorem Natural.from_reduce {a: Aexp} (h: a⇓s = n): s ⊢ a ⟹ n :=
   by induction a generalizing n with
-  | val _ => exact h ▸ Step.val
-  | var _ => exact h ▸ Step.var
-  | add _ _ l r => exact h ▸ Step.add (l rfl) (r rfl)
+  | val _ => exact h ▸ step.val
+  | var _ => exact h ▸ step.var
+  | add _ _ l r => exact h ▸ step.add (l rfl) (r rfl)
 
-@[simp] theorem Step_iff_reduce: (s ⊢ a ⟹ n) ↔ a⇓s = n := ⟨reduce.from_natural, Natural.from_reduce⟩
-@[simp] theorem Step_iff_reduce': s ⊢ a ⟹ (a⇓s) := Natural.from_reduce rfl
+@[simp] theorem step_iff_reduce: (s ⊢ a ⟹ n) ↔ a⇓s = n := ⟨reduce.from_natural, Natural.from_reduce⟩
+@[simp] theorem step_iff_reduce': s ⊢ a ⟹ (a⇓s) := Natural.from_reduce rfl
 
-protected instance Step.equiv: Setoid Aexp where
+protected instance step.equiv: Setoid Aexp where
   r a b := ∀ s n, (s ⊢ a ⟹ n) = (s ⊢ b ⟹ n)
   iseqv := {
     refl := λ _ _ _ ↦ Eq.refl _
@@ -50,12 +50,12 @@ instance reduce.equiv: Setoid Aexp where
   r a b := ∀s, a⇓s = b⇓s
   iseqv := ⟨λ _ _ ↦ Eq.refl _, (Eq.symm $ · ·) , λ h₁ h₂ s ↦ (h₁ s) ▸ (h₂ s)⟩
 
-protected theorem Step_eq_eq_reduce_eq: Step.equiv.r a b ↔ reduce.equiv.r a b := by
+protected theorem step_eq_eq_reduce_eq: step.equiv.r a b ↔ reduce.equiv.r a b := by
   constructor <;> intro h
   . simp [Setoid.r] at *
     intro s
-    specialize h s
-    exact h
+    specialize h s (b⇓s)
+    rw [h]
   . simp [Setoid.r] at *
     simp [h]
 
