Semantics/Imp/Untyped/Structural.lean
@@ -6,27 +6,27 @@ namespace Com
 namespace Structural
 
 @[reducible]
-inductive Step: Com × State → Com × State → Prop where
+inductive step: Com × State → Com × State → Prop where
   | ass:
-    Step (ass x a, s) (skip, s⟪x ≔ a.reduce s⟫)
+    step (ass x a, s) (skip, s⟪x ≔ a⇓s⟫)
 
   | cat₁:
-    Step (skip;;c, s) (c, s)
+    step (skip;;c, s) (c, s)
 
-  | cat₂ (h: Step (c, s) (e, t)):
-    Step (c;;d, s) (e;;d, t)
+  | cat₂ (h: step (c, s) (e, t)):
+    step (c;;d, s) (e;;d, t)
 
   | cond:
-    Step (cond b c d, s) (bif b.reduce s then c else d, s)
+    step (cond b c d, s) (bif b⇓s then c else d, s)
 
   | loop:
-    Step (loop b c, s) (bif b.reduce s then c;;loop b c else skip, s)
+    step (loop b c, s) (bif b⇓s then c;;loop b c else skip, s)
 
-infix:110 " ⇒ " => Step
+infix:110 " ⇒ " => step
 
-theorem Step.demo₁:
-  (⦃x = 0; while x <= 2 {x = x + 1}⦄, ⟪⟫) ⇒
-      (⦃skip; while x <= 2 {x = x + 1}⦄, ⟪⟫⟪"x"≔0⟫) := cat₂ ass
+theorem step.demo₁:
+  (⦃x = 0; while x <= 2 {x = x + 1}⦄, σ₀) ⇒
+      (⦃skip; while x <= 2 {x = x + 1}⦄, σ₀⟪"x" ≔ 0⟫) := cat₂ ass
 
 @[simp] theorem cat_iff:
   (c₁;;c₂, s) ⇒ et ↔
@@ -40,48 +40,48 @@ theorem Step.demo₁:
     | inl h =>
       cases h with | intro e h =>
         cases h with | intro t h =>
-          exact h.right ▸ Step.cat₂ h.1
+          exact h.right ▸ step.cat₂ h.1
     | inr h =>
       cases h with | intro h₁ h₂ =>
-        exact h₁ ▸ h₂ ▸ Step.cat₁
+        exact h₁ ▸ h₂ ▸ step.cat₁
 
 @[simp] lemma cond_iff:
   (cond b c d, s) ⇒ ss ↔
-  (b.reduce s ∧ ss = (c, s)) ∨ (b.reduce s = false ∧ ss = (d, s)) := by
+  (b⇓s ∧ ss = (c, s)) ∨ (b⇓s = false ∧ ss = (d, s)) := by
   constructor <;> intro h
-  . cases hb: b.reduce s <;> cases h
+  . cases hb: b⇓s <;> cases h
     . exact Or.inr ⟨rfl, hb ▸ rfl⟩
     . exact Or.inl ⟨rfl, hb ▸ rfl⟩
-  . have hss: ss = (bif b.reduce s then c else d, s) := by
-      cases hb: b.reduce s <;> rw [hb] at h <;> simp at * <;> assumption
-    exact hss ▸ Step.cond
+  . have hss: ss = (bif b⇓s then c else d, s) := by
+      cases hb: b⇓s <;> rw [hb] at h <;> simp at * <;> assumption
+    exact hss ▸ step.cond
 
-@[simp] lemma cond_false {b: Bexp} (hb: b.reduce s = false):
+@[simp] lemma cond_false {b: Bexp} (hb: b⇓s = false):
   (cond b c d, s) ⇒ ss ↔ (ss = (d, s)) :=
   by rw [cond_iff, hb]; simp
 
-infix:110 " ⇒* " => Relation.ReflTransGen Step
+infix:110 " ⇒* " => Relation.ReflTransGen step
 
-theorem Star.demo₂:
-  (⦃x = 2; while 0 <= x {x = x + 1}⦄, ⟪⟫) ⇒*
-      (⦃while 0 <= x {x = x + 1}⦄, ⟪⟫⟪"x"≔2⟫) :=
-  Relation.ReflTransGen.head (Step.cat₂ Step.ass) (Relation.ReflTransGen.head Step.cat₁ Relation.ReflTransGen.refl)
+theorem star.demo₂:
+  (⦃x = 2; while 0 <= x {x = x + 1}⦄, σ₀) ⇒*
+      (⦃while 0 <= x {x = x + 1}⦄, σ₀⟪"x" ≔ 2⟫) :=
+  Relation.ReflTransGen.head (step.cat₂ step.ass) (Relation.ReflTransGen.head step.cat₁ Relation.ReflTransGen.refl)
 
-theorem Star.cat_skip_cat
+theorem star.cat_skip_cat
   (h: (c, s) ⇒* (skip, t)):
   (c;;d, s) ⇒* (skip;;d, t) :=
-  Relation.ReflTransGen.lift (λ (x: Com × State) ↦ (x.1;;d, x.2)) (λ _ _ h => Step.cat₂ h) h
+  Relation.ReflTransGen.lift (λ (x: Com × State) ↦ (x.1;;d, x.2)) (λ _ _ h => step.cat₂ h) h
 
-theorem Star.cat
+theorem star.cat
   (h₁: (c₁, s) ⇒* (skip, s₁))
   (h₂: (c₂, s₁) ⇒* (skip, s₂)):
   (c₁;;c₂, s) ⇒* (skip, s₂) :=
-  Relation.ReflTransGen.trans (cat_skip_cat h₁) (Relation.ReflTransGen.trans (Relation.ReflTransGen.single Step.cat₁) h₂)
+  Relation.ReflTransGen.trans (cat_skip_cat h₁) (Relation.ReflTransGen.trans (Relation.ReflTransGen.single step.cat₁) h₂)
 
-theorem Star.cat_no_influence
+theorem star.cat_no_influence
   (h: (c₁, s) ⇒* (skip, s₁)):
   (c₁;;c₂, s) ⇒* (c₂, s₁) :=
-  Relation.ReflTransGen.trans (cat_skip_cat h) (Relation.ReflTransGen.single Step.cat₁)
+  Relation.ReflTransGen.trans (cat_skip_cat h) (Relation.ReflTransGen.single step.cat₁)
 
 end Structural
 end Com
