Semantics/Imp/Untyped/Equivalence.lean
@@ -7,28 +7,28 @@ namespace Com
 theorem Structural.from_natural {c: Com} (h: w ⊢ c ⟹ s): (c, w) ⇒* (skip, s) := by
   induction h with
   | skip => exact Relation.ReflTransGen.refl
-  | ass => exact Relation.ReflTransGen.single Step.ass
-  | cat _ _ _ ihc ihd => exact Star.cat ihc ihd
-  | cond₁ hb _ ih => exact Relation.ReflTransGen.head Step.cond (hb ▸ ih)
-  | cond₂ hb _ ih => exact Relation.ReflTransGen.head Step.cond (hb ▸ ih)
+  | ass => exact Relation.ReflTransGen.single step.ass
+  | cat _ _ _ ihc ihd => exact star.cat ihc ihd
+  | cond₁ hb _ ih => exact Relation.ReflTransGen.head step.cond (hb ▸ ih)
+  | cond₂ hb _ ih => exact Relation.ReflTransGen.head step.cond (hb ▸ ih)
   | loop₁ _ hb _ _ ihc ihw =>
-    exact Relation.ReflTransGen.head Step.loop $ Relation.ReflTransGen.trans (hb ▸ Star.cat ihc ihw) Relation.ReflTransGen.refl
+    exact Relation.ReflTransGen.head step.loop $ Relation.ReflTransGen.trans (hb ▸ star.cat ihc ihw) Relation.ReflTransGen.refl
   | loop₂ hb =>
-    exact Relation.ReflTransGen.head Step.loop $ hb ▸ Relation.ReflTransGen.refl
+    exact Relation.ReflTransGen.head step.loop $ hb ▸ Relation.ReflTransGen.refl
 
 lemma Natural.from_structural_step (h₁: x ⇒ y) (h₂: y.2 ⊢ y.1  ⟹ s): x.2 ⊢ x.1 ⟹ s := by
   induction h₁ generalizing s with
-  | ass => exact (skip_iff.mp h₂) ▸ Step.ass
-  | cat₁ => exact Step.cat _ Step.skip h₂
+  | ass => exact (skip_iff.mp h₂) ▸ step.ass
+  | cat₁ => exact step.cat _ step.skip h₂
   | cat₂ _ ih =>
     cases h₂ with
-    | cat w hc hd => exact Step.cat w (ih hc) hd
+    | cat w hc hd => exact step.cat w (ih hc) hd
   | cond => rw [cond_iff']; exact h₂
   | loop => rw [loop_unfold, cond_iff']; exact h₂
 
 theorem Natural.from_structural (h: x ⇒* (skip, t)): x.2 ⊢ x.1 ⟹ t := by
   induction h using Relation.ReflTransGen.head_induction_on with
-  | refl => exact Step.skip
+  | refl => exact step.skip
   | head h _ ht => exact from_structural_step h ht
 
 theorem structural_iff_natural: (c, s) ⇒* (skip, t) ↔ (s ⊢ c ⟹ t) := ⟨Natural.from_structural, Structural.from_natural⟩
@@ -46,21 +46,21 @@ theorem denote.from_natural {c: Com} (h: s ⊢ c ⟹ t): (s, t) ∈ ⟦c⟧ := b
 theorem Natural.from_denote (h: (s, t) ∈ ⟦c⟧): s ⊢ c ⟹ t := by
   revert h
   induction c generalizing s t with
-  | skip => intro h; cases h; exact Step.skip
-  | ass => intro h; simp [denote] at h; exact h ▸ Step.ass
+  | skip => intro h; cases h; exact step.skip
+  | ass => intro h; simp [denote] at h; exact h ▸ step.ass
   | cat _ _ ih₁ ih₂ =>
     intro h
     cases h with | intro w h =>
-      exact Step.cat w (ih₁ h.left) (ih₂ h.right)
+      exact step.cat w (ih₁ h.left) (ih₂ h.right)
   | cond _ _ _ ih₁ ih₂ =>
     intro h
     cases h with
     | inl h =>
       cases h with | intro h hb =>
-        exact Step.cond₁ hb (ih₁ h)
+        exact step.cond₁ hb (ih₁ h)
     | inr h =>
       cases h with | intro h hb =>
-        exact Step.cond₂ hb (ih₂ h)
+        exact step.cond₂ hb (ih₂ h)
   | loop b c ih =>
     suffices ⟦loop b c⟧ ⊆ {s | s.1 ⊢ loop b c ⟹ s.2} by apply this
     apply OrderHom.lfp_le
@@ -70,11 +70,11 @@ theorem Natural.from_denote (h: (s, t) ∈ ⟦c⟧): s ⊢ c ⟹ t := by
       | inl h =>
         cases h with | intro h hb =>
           cases h with | intro w h =>
-            exact Step.loop₁ w hb (ih h.left) h.right
+            exact step.loop₁ w hb (ih h.left) h.right
       | inr h =>
         cases h with | intro hq hb =>
           simp at hq
-          exact hq ▸ Step.loop₂ hb
+          exact hq ▸ step.loop₂ hb
 
 theorem natural_iff_denote: (s, t) ∈ ⟦c⟧ ↔ (s ⊢ c ⟹ t) := ⟨Natural.from_denote, denote.from_natural⟩
 
