Semantics/Maps.lean
@@ -1,0 +1,32 @@
+/-
+# Maps
+-/
+
+/-
+## Total maps
+-/
+
+def total_map A := String → A
+
+def total_map.default (v: A): total_map A := λ _ ↦ v
+
+def total_map.update (m: total_map A) (x: String) (v: A) :=
+  λ y ↦ bif x = y then v else m y
+
+notation m "⟪" x " ≔ " v "⟫" => total_map.update m x v
+
+/-
+## Partial maps
+-/
+
+def partial_map A := total_map $ Option A
+
+def partial_map.default: partial_map A := λ _ ↦ none
+
+def includedin (a b: partial_map A) := ∀ x v, (a x = some v) → (b x = some v)
+
+theorem includedin_update x v (h: includedin a b):
+  includedin (a ⟪x ≔ some v⟫) (b ⟪x ≔ some v⟫) :=  by
+  {
+    sorry
+  }
